\section{Basics}
$f(x) = \frac{1}{\sqrt{2\pi \sigma^2}} e^{- \frac{1}{2} \frac{(x-\mu)^2}{\sigma^2}},\quad \mathcal{N}(x|\mu, \sigma)$\\
$f(x) = \frac{1}{\sqrt{(2\pi)^d\det\Sigma}} e^{- \frac{1}{2} (x-\mu)^T \Sigma^{-1} (x-\mu)},\quad \mathcal{N}(x|\mu, \Sigma)$\\
% Condition number: $\kappa(A)=\frac{\sigma_{max}(A)}{\sigma_{min}(A)}$ \\
% Binomial: $f(k,n,p) {=} Pr(X=k) {=} \binom nk p^k (1{-}p)^{n{-}k}$ \\
% $\ln(\mathcal{N}(x|\mu, \Sigma)) {=} {-}\tfrac{d}{2}\ln(2\pi) {-} \tfrac{\ln|\Sigma|}{2} {-} \tfrac{1}{2}(x{-}\mu)^T\Sigma(x{-}\mu)$ \\
$X {\sim} \mathcal{N}(\mu,\Sigma)$, $Y{=}A{+}BX \Rightarrow Y{\sim}\mathcal{N}(A{+}B\mu,B\Sigma B^T)$

$log(\mathcal{N}(x|\mu, \Sigma)) = \frac{1}{2}log|\Sigma^{-1}|- \frac{1}{2}(x - \mu)^T\Sigma^{-1}(x - \mu) + const \Rightarrow \frac{\partial log\mathcal{N}(x|\mu, \Sigma)}{\mu} = \Sigma^{-1}(x - \mu)$, $\frac{\partial log\mathcal{N}(x|\mu, \Sigma)}{\Sigma^{-1}} = \frac{1}{2}\Sigma - \frac{1}{2}(x - \mu)(x - \mu)^T$
% Derivation: let $\wedge = \Sigma^{-1}$, $\frac{\partial}{\partial \wedge} (x - \mu)^T \wedge (x - \mu) = \frac{\partial}{\partial \wedge} Tr(x - \mu) (x - \mu)^T \wedge)$

f(x) on a: $f(a)+\tfrac{f'(a)}{1!}(x-a) + \tfrac{f''(a)} {2!}(x-a)^2 + ...$ \\

% Cond. Gaussian: 
$p(\begin{bmatrix}a_1\\a_2\end{bmatrix}) = \mathcal{N}(\begin{bmatrix}u_1\\u_2\end{bmatrix}, \begin{bmatrix}\Sigma_{11} \Sigma_{12}\\ \Sigma_{21} \Sigma_{22}\end{bmatrix})$,
$p(a_2 | a_1) = \mathcal{N}(u_2 + \Sigma_{21}\Sigma_{11}^{-1}(a_1-u_1), \Sigma_{22}-\Sigma_{21}\Sigma_{11}^{-1}\Sigma_{12})$
% General p-norm: $\norm{ x }_p = (\sum_{i=1}^n |x_i|^p)^{1/p}$
\\
% \subsection*{Moments}
% \item{\textbf{Moments:}}
% \textbf{Moments: } 
\begin{inparaitem}[\color{red}\textbullet]
% Variance
\item $Var[X]=\int_x(x-\mu)^2p(x) dx$\\
\item $Var[aX]=a^2Var[X]$\\
\item $Var[X]=E[(X-E[X])^2]=E[X^2]-E[X]^2$ \\
\item $Var[X{+}Y]=Var[X]{+}Var[Y]{+}2Cov[X,Y]$ \\
% Covariance
\item $Cov[X,Y] = E[(X - E[X])(Y - E[Y])]$ \\
\item $Cov[aX,bY]{=}abCov[X,Y]$
% \item $K_{\bm{XY}} = cov(X,Y) = E[XY^T] - E[X]E[Y^T]$
% \end{inparaitem}
% \subsection*{Calculus}
% \item{\textbf{Calculus:}}
% \textbf{Calculus: } 
% \begin{inparaitem}[\color{red}\textbullet]
	% \item Part.: $\int u(x)v'(x) dx = u(x)v(x) - \int v(x)u'(x) dx$\\
	% \item Chain r.: $\frac{f(y)}{g(x)} = \frac{dz}{dx} \Big|_{x=x_0}= \frac{dz}{dy}\Big|_{z=g(x_0)}\cdot \frac{dy}{dx} \Big|_{x=x_0}$ \\
	%\item $g_x(1) = g_x(0) + g'_x(0) + \int_{0}^{1} g_x''(s)(1-s) ds$ \\
	%\item $g(\mathbf{w}+\delta) - g(\mathbf{w}) = %\int_{\mathbf{w}}^{\mathbf{w+\delta}} \nabla g(\mathbf{u}) du = (\int_{0}^{1} \nabla g(\mathbf{w}+t\delta)dt) \cdot \delta$\\
	\item $\frac{\partial}{\partial \mathbf{x}}(\mathbf{b}^\top \mathbf{x}) = \frac{\partial}{\partial \mathbf{x}}(\mathbf{x}^\top \mathbf{b}) = \mathbf{b}$
	\item $\frac{\partial}{\partial \mathbf{x}}(\mathbf{x}^\top \mathbf{x}) = 2\mathbf{x}$ \\
	\item $\frac{\partial}{\partial \mathbf{x}}(\mathbf{x}^\top \mathbf{A}\mathbf{x}) = (\mathbf{A}^\top + \mathbf{A})\mathbf{x} \stackrel{\text{\tiny A sym.}}{=} 2\mathbf{A}\mathbf{x}$ \\
	\item $\frac{\partial}{\partial \mathbf{x}}(\mathbf{b}^\top \mathbf{A}\mathbf{x}) = \mathbf{A}^\top \mathbf{b}$
	\item $\frac{\partial}{\partial \mathbf{X}}(\mathbf{c}^\top \mathbf{X} \mathbf{b}) = \mathbf{c}\mathbf{b}^\top$ \\
	\item $\frac{\partial}{\partial \mathbf{X}}(\mathbf{c}^\top \mathbf{X}^\top \mathbf{b}) = \mathbf{b}\mathbf{c}^\top$
	\item $\frac{\partial}{\partial \mathbf{x}}(\| \mathbf{x}-\mathbf{b} \|_2) = \frac{\mathbf{x}-\mathbf{b}}{\|\mathbf{x}-\mathbf{b}\|_2}$ \\
	% \item $\frac{\partial}{\partial \mathbf{x}}(\|\mathbf{x}\|^2_2) = \frac{\partial}{\partial \mathbf{x}} (\|\mathbf{x}^\top \mathbf{x}\|_2) = 2\mathbf{x}$
	% \item $\frac{\partial}{\partial \mathbf{X}}(\|\mathbf{X}\|_F^2) = 2\mathbf{X}$ \\
	\item $x^T A x = Tr(x^T A x) = Tr(x x^T A) = Tr(A x x^T)$ \\
	\item $\tfrac{\partial}{\partial A} Tr(AB) {=} B^T$
	\item $\frac{\partial}{\partial A} log|A| {=} A^{-T}$ \\
	\item $\text{sigmoid}(x) = \sigma(x) = \frac{1}{1+\exp(-x)}$ \\
	\item $\nabla \text{sigmoid}(x) = \text{sigmoid}(x)(1-\text{sigmoid}(x))$
	% \item $\nabla \text{tanh}(x) = 1-\text{tanh}^2(x)$ 
	% \item $tanhx {=} \frac{sinhx}{coshx} {=} \frac{e^{x}-e^{-x}}{e^{x} + e^{x}}$
\end{inparaitem}
% \subsection*{Bayes' Rule}
% $ P(Y|X) = \frac{P(X|Y)P(Y)}{P(X)}\frac{P(X|Y)P(Y)}{\sum\limits^k_{i=1}P(X|Y_i)P(Y_i)}$\\
	% \item[MGF] $\mathbf{M}_X(t)=\mathbb{E}[e^{\mathbf{t}^T \mathbf{X}}]$, $\mathbf{X}=(X_1,.., X_n) $
% \subsection*{Expected Risk}
% $R(f, X) = \int_{y}Q(Y, f(X))P(Y|X)dY$ \\
% $R(f) = \mathbb{E}_{X}[R(f, X)] = \int_{X}R(f, X)P(X)dX = \int_y\int_xQ(Y, f(X))P(X, Y)dX dY$
% \subsection*{Jensen's inequality}
% 	X:random variable \& $\varphi$:convex function $\rightarrow$ $\varphi(\mathbb{E}[X]) \leq \mathbb{E}[\varphi(X)]$
% \subsection*{Cauchyâ€“Schwarz inequality}
% $|\langle u, v \rangle^2| \leq \langle u, u \rangle \cdot \langle v, v \rangle$